theories/equivalence/LanguagesUtils.v
@@ -51,6 +51,7 @@ Definition incr_string {n : nat} (s : StringLang.string n) : (StringLang.string 
   ++ reflexivity.
 Defined.
 
+
 Extraction incr_string.
 
 
